library/data/rbmap/default.lean
@@ -59,9 +59,9 @@ end
 
 lemma eq_some_of_to_value_eq_some {e : option (α × β)} {v : β} : to_value e = some v → ∃ k, e = some (k, v) :=
 begin
-  cases e; simp [to_value],
+  cases e with val; simp [to_value],
     { contradiction },
-    { cases a, simp, intro h, injection h, subst v, existsi fst, refl }
+    { cases val, simp, intro h, injection h, subst v, existsi fst, refl }
 end
 
 lemma eq_none_of_to_value_eq_none {e : option (α × β)} : to_value e = none → e = none :=
